\documentclass{article}
\title{QM HW1}
\author{Jiete XUE}
\date{2025/09/02}
\usepackage{amsthm}
\newtheoremstyle{t}{0pt}{}{}{}{\bfseries}{}{\newline}{}
\theoremstyle{t}
\newtheorem{problem}{Problem}
\usepackage{chngcntr}
\counterwithin{equation}{problem}
\newcommand{\dd}{\mathrm{d}}
\newcommand{\pa}{\partial}
\begin{document}

\maketitle
\begin{problem}[Canonical Transformation]
(1)\begin{equation}
   \dd \Phi(q,P,t)=p\dd q+Q\dd P+(H'-H)\dd t 
\end{equation}
\begin{equation}
    \frac{\partial \Phi}{\partial q}=p,\frac{\partial \Phi}{\partial P}=Q,\frac{\partial \Phi}{\partial t}+H=H'.
\end{equation}
(2) We have proved:
\begin{equation}
    \frac{\partial S}{\partial q_t}=-p_t,\frac{\partial S}{\partial q_{t+\tau}}=p_{t+\tau},
\end{equation}
First, we can check:
\begin{equation}
    \frac{\partial \Psi}{\partial q_t}=-\frac{\partial S}{\partial q_t}=p_t
\end{equation}
Second ,by chain rule,we obtain
\begin{equation}
    \frac{\partial \Psi }{\partial p_{t+\tau}}=q_{t+\tau}+\left( p_{t+\tau}-\frac{\partial S}{\partial p_{t+\tau}}\right)\frac{\partial q_{t+\tau}}{\partial p_{t+\tau}}=q_{t+\tau}
\end{equation}
(3) \begin{equation}
    \dd p_t\wedge\dd q_t=\dd p_{t+\tau}\wedge\dd q_{t+\tau},\frac{\partial(q_{t+\tau},p_{t+\tau})}{\partial(q_t,p_t)}=1
\end{equation}
\end{problem}
\begin{problem}[Hamilton-Jacobi equation]
    (1) \begin{equation}
        \frac{\pa S}{\pa t}=\frac{\dd S}{\dd t}-\frac{\pa S}{\pa q}\dot{q}=L-p\dot{q}=-H
    \end{equation}
    (2) \begin{equation}
        \beta=\frac{\pa S}{\pa \alpha}
    \end{equation}
    \begin{equation}
        H'=H+\frac{\pa S}{\pa t}=0
    \end{equation}
\end{problem}
\begin{problem}[Harmonic Oscillator]
    (1) easy to check:
    \begin{equation}
        \frac{\pa S}{\pa x}=p,\frac{\pa S}{\pa t}=-E
    \end{equation}
    (2)\begin{equation}
        \frac{\pa S}{\pa t_f}=-E
    \end{equation}
    \begin{equation}
        \frac{\pa S}{\pa x_f}=p=\pm m \omega \sqrt{A^2-x^2}
    \end{equation}
    (3)
    \begin{equation}
        S=\pm m \omega \int \sqrt{\frac{2E}{m \omega^2}-x^2}\, \dd x-E t+\mathrm{const.}
    \end{equation}
    \begin{equation}
        \frac{\pa S}{\pa E}=\pm \frac{\arcsin (\sqrt{\frac{m \omega^2}{2E}}x)}{\omega}-t
    \end{equation}
    New Hamitonian:
    \begin{equation}
        H'=H+\frac{\pa S}{\pa t}=0
    \end{equation}
    By Hamilton equation
    \begin{equation}
        \dot{\beta}=\frac{\pa H'}{\pa E}=0
    \end{equation}
    Therefore $\beta$ is a constant.It means the initial phase of  oscillator.
\end{problem}
\begin{problem}[Planck’s derivation of black body radiation]
    Confused.
\end{problem}
\begin{problem}[Heisenberg’s magic]

\end{problem}
\end{document}